@prefix konig: <http://www.konig.io/ns/core/> .
@prefix owl: <http://www.w3.org/2002/07/owl#> .
@prefix sh: <http://www.w3.org/ns/shacl#> .
@prefix rdf: <http://www.w3.org/1999/02/22-rdf-syntax-ns#> .
@prefix rdfs: <http://www.w3.org/2000/01/rdf-schema#> .
@prefix vann: <http://purl.org/vocab/vann/> .
@prefix schema: <http://schema.org/> .
@prefix xsd: <http://www.w3.org/2001/XMLSchema#> .

konig: a owl:Ontology ;
	rdfs:label "Konig Core Ontology" ;
	rdfs:comment """Provides terms that extend OWL and SHACL.
		<p>A description of this ontology in Turtle syntax is available at 
		<a href="http://www.konig.io/ns/kol/.ttl">http://www.konig.io/ns/core/.ttl</a></p>""" ;
	vann:preferredNamespacePrefix "kol"
	.


###### Generic Data Modeling Terms
		

konig:id a owl:DatatypeProperty, owl:FunctionalProperty ;
	rdfs:comment """
		A pseudo-property whose value is equal to the IRI used to identify the subject.
		We call it a "pseudo-property" because (by convention) neither OWL nor SHACL models 
		expect an explicit property for the IRI value.  Instead, an OWL model may declare a class
		to be a subclass of owl:NamedIndividual to indicate that all instances of the class must be
		identified by an IRI.  Similarly, a SHACL model will use
		sh:nodeKind to specify whether a given entity is identified by an IRI or a BlankNode.
		These OWL and SHACL conventions can be inconvenient.  Sometimes we want to treat the IRI for a resource on 
		equal footing with other properties.  The konig:id property allows us to do that.
		A PropertyConstraint with konig:id as the sh:predicate and sh:minCount equal to 1 
		is equivalent to specifying that sh:nodeKind is sh:IRI on the parent shape.
		A PropertyConstraint with konig:id as the predicate and sh:minCount equal to zero 
		(or undefined) is equivalent to specifying that sh:nodeKind is sh:BlankNodeOrIRI.
	""" ;
	rdfs:range xsd:anyURI
.

konig:JsonSchema a owl:Class ;
	rdfs:comment "The class of all JSON Schema definitions"
.

konig:AvroSchema a owl:Class ;
	rdfs:comment "The class of all Avro Schema definitions"
.

konig:mediaTypeBaseName a owl:DatatypeProperty ;	
	rdfs:domain sh:Shape ;
	rdfs:range xsd:string ;
	rdfs:comment """
		The base name for the vendor-specific media type associated with this Shape.
		The mediaTypeBaseName includes all parts of the media type name except the suffix.
	"""
.

konig:jsonSchemaRendition	a owl:ObjectProperty ;
	rdfs:domain sh:Shape ;
	rdfs:range konig:JsonSchema ;
	rdfs:comment "The JSON Schema rendition of the Shape"
.

konig:avroSchemaRendition	a owl:ObjectProperty ;
	rdfs:domain sh:Shape ;
	rdfs:range konig:AvroSchema ;
	rdfs:comment "The Avro Schema rendition of the Shape"
.

konig:PreferredClass a owl:Class ;
	rdfs:subClassOf owl:Class ;
	rdfs:comment """
		A type value which distinguishes one member from a set of equivalent classes as the
		"preferred" member.  This is useful if you want to provide metaprograms with a 
		hint about which class name to use when generating source code. Technically, the
		concept of a PreferredClass is nonsense.  According to the rules of owl:equivalentClass,
		any property asserted on one member of the equivalence relation applies equally well
		to all other members.
    In other words, if you have the statements (A owl:equivalentClass B) and
		(A rdf:type konig:PreferredClass), then a semantic reasoner can infer
		(B rdf:type konig:PreferredClass).  Nevertheless, this construct is useful so long
		as the metaprogram captures the PreferredClass distinction before applying any 
		semantic reasoning.
	"""
.	

konig:equivalentPath a owl:DatatypeProperty ;
	rdfs:comment """
		A string value that describes a path from the focus node to a value that is equal to the
		value of the property described by this PropertyConstraint.
	""" ;
	rdfs:domain sh:PropertyConstraint ;
	rdfs:range xsd:string
.	
	
###### GraphDiff terms

konig:GraphDiff a owl:Class ;
	rdfs:subClassOf konig:Graph ;
	rdfs:comment """
		A collection of annotated statements that prescribe the delta between two versions of some
		graph.
	"""
	.

konig:Dictum a owl:Class ;
	rdfs:subClassOf rdf:Statement ;
	rdfs:comment """
		A Statement that is known to be true. A semantic reasoner may convert individual 
		Dictum statements into simple (non-reified) triples of the form (subject predicate object). 
		Dictum statements are included in a konig:GraphDiff to describe statements that must be
		added to the source graph to produce the target revision. 
	"""
.

konig:Falsehood a owl:Class ;
	rdfs:subClassOf rdf:Statement ;
	rdfs:comment """
		A Statement that is known to be false. A semantic reasoner should remove any Triple that is
		defined as a Falsehood.  Falsehood statements are included in a konig:GraphDiff to define
		statements that must be removed from the source graph to produce the target revision. 
	"""
.

konig:KeyValue a owl:Class ;
	rdfs:subClassOf rdf:Statement ;
	rdfs:comment """
		A Statement which asserts that the (predicate object) pair is a unique key for
		the subject.
	"""
.

konig:KeyTerm a owl:Class ;
	rdfs:subClassOf rdf:Statement ;
	rdfs:comment """
		A reified Statement which asserts that the predicate is a unique key for the subject.
	"""
.

###### Data Generator Terms

konig:SyntheticGraphConstraints a owl:Class ;
	rdfs:comment """
		Constraints on the structure of a synthetic graph.  This resource is used by 
		tools that generate synthetic graphs for testing purposes.
	"""
.

konig:SyntheticClassConstraints a owl:Class ;
	rdfs:comment """
		A resource that governs the generation of synthetic instances of a given
		OWL Class for testing purposes.
	"""
.	

konig:SyntheticShapeConstraints a owl:Class ;
	rdfs:comment """
		A resource that governs the generation of synthetic instances of a given 
		data shape for testing purposes.
	"""
.	

konig:classConstraints a owl:ObjectProperty ;
	rdfs:comment """
		A constraint on instances of a given OWL Class within the synthetic graph
	""" ;
	rdfs:domain konig:SyntheticGraphConstraints ;
	rdfs:range konig:SyntheticClassConstraints
.

konig:constrainedClass a owl:ObjectProperty ;
	rdfs:comment "The class that is being constrained." ;
	rdfs:domain konig:SyntheticClassConstraints ;
	rdfs:range owl:Class
.

konig:shapeConstraints a owl:ObjectProperty ;
	rdfs:comment """
		A constraint on instances of a given Shape within the synthetic graph
	""" ;
	rdfs:domain konig:SyntheticGraphConstraints ;
	rdfs:domain konig:SyntheticShapeConstraints
.

konig:constrainedShape a owl:ObjectProperty ;
	rdfs:comment "The Shape that is being constrained." ;
	rdfs:domain konig:SyntheticShapeConstraints ;
	rdfs:range sh:Shape
.

konig:classInstanceCount a owl:DatatypeProperty ;
	rdfs:comment "The number of instances of the class to be generated" ;
	rdfs:domain konig:SyntheticClassConstraints ;
	rdfs:range xsd:int
.

konig:shapeInstanceCount a owl:DatatypeProperty ;
	rdfs:comment "The number of instances of the shape to be generated" ;
	rdfs:domain konig:SyntheticShapeConstraints ;
	rdfs:range xsd:int
.	

	
###### Fact Modeling

konig:Fact a owl:Class ;
	rdfs:comment "The class of all facts.  Each fact has a measure and some dimensions." 
.	

konig:TimeInterval a owl:Class ;
	rdfs:comment "An interval of time that has an explicit starting point and a duration"
.	

konig:TimeUnit a owl:Class ;
	rdfs:subClassOf owl:NamedIndividual ;
	rdfs:comment "The class of all possible time unit values (Day, Week, Month, Year, etc.)" 
.

konig:Week a konig:TimeUnit ;	
	rdfs:comment "A unit of time that is one week in duration"
.

konig:Month a konig:TimeUnit ;
	rdfs:comment "The unit of time that is one month in duration"
.

konig:Year a konig:TimeUnit ;
	rdfs:comment "The unit of time that is one year in duration"
.

konig:measure a owl:ObjectProperty ;
	rdfs:subPropertyOf sh:predicate ;
	rdfs:comment "A predicate whose value is an observed or computed measure."
.	

konig:dimension a owl:ObjectProperty ;
	rdfs:subPropertyOf sh:predicate ;
	rdfs:comment "A predicate whose value is one dimension of a fact"
.

konig:attribute a owl:ObjectProperty ;
	rdfs:subPropertyOf sh:predicate ;
	rdfs:comment "A predicate whose value is an attribute of some dimension"
.

konig:stereotype a owl:ObjectProperty ;
	rdfs:comment """
		An annotation on a PropertyConstraint which identifies the role of the property
		in some external framework.  By "external" we mean external to the SHACL vocabulary.
		A stereotype allows one to understand how the property will be used.  In this sense,
		it is similar to a UML stereotype (hence the name).  As an example, one could use stereotypes
		to distinguish measures, dimensions and attributes in an OLAP cube.
	""" ;
	rdfs:domain sh:PropertyConstraint ;
	rdfs:range rdf:Property
.	


konig:totalCount a owl:DatatypeProperty ;
	rdfs:comment """
		A measure which records the total number of times that some data Shape
		occurs.
	""" ;
	rdfs:domain konig:Fact ;
	rdfs:range xsd:int
.

konig:durationUnit a owl:ObjectProperty ;
	rdfs:comment "The unit of time used to define the duration of the TimeInterval" ;
	rdfs:domain konig:TimeInterval ;
	rdfs:range konig:TimeUnit
.	

konig:intervalStart a owl:ObjectProperty ;
	rdfs:comment "The point in time when the interval started." ;
	rdfs:domain konig:TimeInterval ;
	schema:rangeIncludes xsd:date , xsd:dateTime
.	
		
konig:inputClass a owl:ObjectProperty ;
	rdfs:comment "The class of entities from which instances of this Shape are derived." ;
	rdfs:domain sh:Shape ;
	rdfs:range owl:Class
.	
